systems/chord-props/HashInjective.v
@@ -1,0 +1,37 @@
+Require Import List.
+Import ListNotations.
+
+Require Import StructTact.StructTactics.
+Require Import StructTact.Util.
+
+Require Import Chord.Chord.
+Require Import Chord.SystemReachable.
+
+Set Bullet Behavior "Strict Subproofs".
+
+Lemma nodes_same_hash_still_injective :
+  forall gst gst',
+    nodes gst = nodes gst' ->
+    hash_injective_on gst ->
+    hash_injective_on gst'.
+Proof.
+  unfold hash_injective_on.
+  intros; repeat find_rewrite; auto.
+Qed.
+Hint Resolve nodes_same_hash_still_injective.
+
+Theorem hash_injective_invariant :
+  forall gst,
+    reachable_st gst ->
+    hash_injective_on gst.
+Proof.
+  eapply chord_net_invariant; do 2 autounfold; intros;
+    try solve [inv_prop initial_st; tauto
+              |eapply nodes_same_hash_still_injective; try eassumption;
+               subst; auto].
+  unfold hash_injective_on, start_constraint in *; intros.
+  repeat find_rewrite; in_crush;
+    exfalso; find_eapply_prop hash;
+      solve [repeat find_rewrite; now apply in_map
+            |repeat find_reverse_rewrite; now apply in_map].
+Qed.
